fixed alert state, will work on script to test

Dafny/Alert.dfy
@@ -1,9 +1,30 @@
-include "BloodInventory.dfy"
 class Alert
 {
+    var alertOn: bool
+
+    predicate Valid()
+    reads this
+    {
+        true
+    }
+
+    constructor()
+    modifies this
+    ensures !alertOn
+    ensures Valid()
+    {
+        alertOn := false;
+    }
+
     method CheckForAlert(threshold: int, countForBloodType: int) returns (alert: bool)
     ensures alert == (threshold >= countForBloodType)
     {
         alert := (threshold >= countForBloodType);
+    }
+
+    function method IsAlertOn(): bool
+    reads this
+    {
+        alertOn
     }
 } // end of Alert class
